NCML.lean
@@ -1,5 +1,7 @@
 module  -- shake: keep-all --deprecated_module: ignore
 
+public import NCML.CK.Axioms.BBox
+public import NCML.CK.Axioms.BDia
 public import NCML.CK.Axioms.D
 public import NCML.CK.Axioms.TBox
 public import NCML.CK.Axioms.TDia
