NCML/CK/Axioms/BDia.lean
@@ -1,0 +1,85 @@
+module
+
+public import NCML.CK.Confluence
+
+@[expose] public section
+
+namespace CK
+
+variable {κ : Type*}
+variable {A : BDFormula}
+
+namespace Frame
+
+variable {F : Frame κ}
+
+/-- The frame condition defined by `B◇`: every world has a `≼`-successor all of whose
+`⊏`-successors return to it, unless it is fallible. -/
+class BDia (F : Frame κ) : Prop where
+  bDia : ∀ x, ¬F.Fallible x → ∃ y, x ≼ y ∧ ∀ z, y ⊏ z → ∃ w v, z ≼ w ∧ w ⊏ v ∧ v ≼ x
+export BDia (bDia)
+
+instance [F.SymmetricMRel] : F.BDia where
+  bDia x _ := by
+    use x;
+    and_intros;
+    . apply refl;
+    . intro z Mxz;
+      use z, x;
+      and_intros;
+      . apply refl;
+      . apply symm_mRel Mxz;
+      . apply refl;
+
+lemma valid_BDia [F.BDia] : F ⊧ (◇(□A) 🡒 A) := by
+  intro V V_per V_fal x y _ hy;
+  by_cases hFallible : F.Fallible y;
+  . exact forces_of_fallible hFallible;
+  . obtain ⟨z, Iyz, hz⟩ := bDia y hFallible;
+    obtain ⟨w, Izw, hw⟩ := hy z Iyz;
+    obtain ⟨v, u, Iwv, Mvu, Iuy⟩ := hz w Izw;
+    exact forces_persistent (hw v u Iwv Mvu) Iuy;
+
+lemma bDia_of_valid_BDia (h : F ⊧ (◇(□(#0)) 🡒 #0)) : F.BDia where
+  bDia x hx := by
+    by_contra! hc;
+    let M : Model κ := {
+      toFrame := F,
+      val := fun y _ => ¬(y ≼ x) ∨ F.Fallible y,
+      val_persistent := by
+        rintro y z a (hy | hy) Iyz;
+        . left;
+          intro hzx;
+          exact hy $ Trans.trans Iyz hzx;
+        . right;
+          exact F.fallible_iRel hy Iyz;
+      fallible_val := by
+        rintro y a hy;
+        right;
+        exact hy;
+    }
+    have hDiaBox : x ⊩[M] ◇(□(#0)) := by
+      intro y Ixy;
+      obtain ⟨z, Myz, hz⟩ := hc y Ixy;
+      refine ⟨z, Myz, ?_⟩;
+      intro w v Izw Mwv;
+      exact Or.inl $ hz w v Izw Mwv;
+    rcases h M.val M.val_persistent M.fallible_val x x (refl x) hDiaBox with hc₁ | hc₁;
+    . exact hc₁ (refl x);
+    . exact hx hc₁;
+
+theorem bDia_TFAE : List.TFAE [
+  F.BDia,
+  ∀ A : BDFormula, F ⊧ (◇(□A) 🡒 A),
+  F ⊧ (◇(□(#0)) 🡒 #0),
+] := by
+  tfae_have 1 → 2 := by intro h A; exact valid_BDia;
+  tfae_have 2 → 3 := fun h => h _
+  tfae_have 3 → 1 := bDia_of_valid_BDia
+  tfae_finish
+
+end Frame
+
+end CK
+
+end
