NCML/CK/Countermodel/BBox.lean
@@ -1,6 +1,6 @@
 module
 
-public import NCML.CK.Confluence
+public import NCML.CK.Axioms.BBox
 
 @[expose] public section
 
@@ -27,30 +27,35 @@ def counterModel : Model (Fin 3) where
 instance : counterModel.SymmetricMRel where
   symm_mRel := by grind [counterModel]
 
-lemma counterModel_not_forwardConfluent : ¬ counterModel.ForwardConfluent := by
+lemma counterModel_not_forwardConfluent : ¬counterModel.ForwardConfluent := by
   rintro ⟨h⟩;
-  obtain ⟨y₁, -, M2y₁⟩ := h (x := 1) (y := 0) (x₁ := 2) (by tauto) (by tauto);
-  simp only [counterModel, Frame.mRel] at M2y₁;
+  obtain ⟨w, -, M2w⟩ := h (x := 1) (y := 0) (z := 2) (by tauto) (by tauto);
+  simp only [counterModel, Frame.mRel] at M2w;
   omega;
 
-lemma counterModel_not_forces :
-    (0 : counterModel.World) ⊮[_] (#0 🡒 □◇(#0)) := by
-  intro h;
-  have h0 : (0 : counterModel.World) ⊩[_] (#0 : BDFormula) := by
-    show counterModel.val 0 0;
-    grind [counterModel];
-  have hbox : (0 : counterModel.World) ⊩[_] □◇(#0) := h 0 (by tauto) h0;
-  have h1 : (1 : counterModel.World) ⊩[_] ◇(#0) := hbox 0 1 (by tauto) (by tauto);
+lemma counterModel_not_bBox : ¬counterModel.BBox := by
+  rintro ⟨h⟩;
+  obtain ⟨w, M2w, -⟩ := h (x := 0) (y := 1) (z := 2) (by tauto) (by tauto);
+  simp [counterModel, Frame.mRel] at M2w;
+
+lemma counterModel_not_forces : 0 ⊮[counterModel] (#0 🡒 □◇(#0)) := by
+  by_contra! h;
+  have h0 : 0 ⊩[counterModel] (#0) := by tauto;
+  have hbox : 0 ⊩[counterModel] □◇(#0) := h 0 (by tauto) h0;
+  have h1 : 1 ⊩[counterModel] ◇(#0) := hbox 0 1 (by tauto) (by tauto);
   obtain ⟨z, M2z, hzA⟩ := h1 2 (by tauto);
-  simp only [counterModel, Frame.mRel] at M2z;
-  omega;
+  simp [counterModel, Frame.mRel] at M2z;
 
 end BBox
 
 /-- - [Pac24, Proposition 9] -/
 theorem exists_symmetricMRel_not_forces_bBox :
-    ∃ (κ : Type) (M : Model κ), M.SymmetricMRel ∧ ∃ x : M.World, x ⊮[_] (#0 🡒 □◇(#0)) :=
+  ∃ (κ : Type) (M : Model κ), M.SymmetricMRel ∧ ∃ x : M.World, x ⊮[_] (#0 🡒 □◇(#0)) :=
   ⟨Fin 3, BBox.counterModel, inferInstance, 0, BBox.counterModel_not_forces⟩
+
+theorem exists_symmetricMRel_not_bBox :
+  ∃ (κ : Type) (F : Frame κ), F.SymmetricMRel ∧ ¬F.BBox :=
+  ⟨Fin 3, BBox.counterModel.toFrame, inferInstance, BBox.counterModel_not_bBox⟩
 
 end CK
 
