NCML/CK/Soundness.lean
@@ -2,6 +2,8 @@ module
 
 public import NCML.CK.Semantics
 public import NCML.CK.Confluence
+public import NCML.CK.Axioms.BBox
+public import NCML.CK.Axioms.BDia
 public import NCML.Hilbert.Logics
 
 @[expose] public section
@@ -11,6 +13,8 @@ namespace CK
 variable {κ : Type*} {M : Model κ}
 
 namespace Model
+
+open CK.Frame
 
 lemma valid_of_mem_logic (h𝔸 : ∀ B ∈ 𝔸, M ⊧ B) (hA : A ∈ ProvableBDHilbert.logic 𝔸) : M ⊧ A := by
   replace hA : ProvableBDHilbert 𝔸 A := hA;
@@ -39,19 +43,19 @@ lemma valid_of_mem_LogicCK (hA : A ∈ LogicCK) : M ⊧ A := valid_of_mem_logic 
 lemma valid_of_mem_LogicCKB [M.IsCKB] (hA : A ∈ LogicCKB) : M ⊧ A :=
   valid_of_mem_logic (by
     rintro B (⟨C, rfl⟩ | ⟨C, rfl⟩);
-    · exact valid_BBox_of_symmetricMRel_of_forwardConfluent;
-    · exact valid_BDia_of_symmetricMRel_of_forwardConfluent;
+    · exact valid_of_toFrame_valid valid_BBox;
+    · exact valid_of_toFrame_valid valid_BDia;
   ) hA
 
 /-- - [Pac24, Lemma 14] -/
 lemma valid_of_mem_LogicIKB [M.IsIKB] (hA : A ∈ LogicIKB) : M ⊧ A :=
   valid_of_mem_logic (by
     rintro B ((((⟨C, D, rfl⟩ | ⟨C, D, rfl⟩) | rfl) | ⟨C, rfl⟩) | ⟨C, rfl⟩);
-    · exact valid_FS_of_forwardConfluent_of_backwardConfluent;
-    · exact valid_DP_of_forwardConfluent;
-    · exact valid_N_of_symmetricMRel;
-    · exact valid_BBox_of_symmetricMRel_of_forwardConfluent;
-    · exact valid_BDia_of_symmetricMRel_of_forwardConfluent;
+    · exact valid_of_toFrame_valid valid_FS_of_forwardConfluent_of_backwardConfluent;
+    · exact valid_of_toFrame_valid valid_DP_of_forwardConfluent;
+    · exact valid_of_toFrame_valid valid_N_of_symmetricMRel;
+    · exact valid_of_toFrame_valid valid_BBox;
+    · exact valid_of_toFrame_valid valid_BDia;
   ) hA
 
 end Model
